\documentclass{minimal}
\usepackage{amsmath}
\begin{document}
Let $\psi = \frac{1 - \sqrt{5}}{2}$ and
\begin{math}
  Fib(n) = 
    \begin{cases}
      0 & \text{if n = 0}\\
      1 & \text{if n = 1}\\
      Fib(n-1) + Fib(n-2) & \text{otherwise}
    \end{cases}
\end{math}

% TODO: prove the hint here

$Fib(n) = \frac{\phi^n - \psi^n}{\sqrt{5}}$:

When $n = 0$, $Fib(0) = 0$ and $\frac{\phi^0 - \psi^0}{\sqrt{5}} =
\frac{1 - 1}{\sqrt{5}} = 0$.

When $n = 1$, $Fib(1) = 1$ and
\begin{eqnarray*}
  \frac{\phi^1 - \psi^1}{\sqrt{5}} &=& \frac{\frac{1 + \sqrt{5} - (1 - \sqrt{5})}{2}}{\sqrt{5}}
                                \\ &=& \frac{2\sqrt{5}}{2\sqrt{5}}
                                \\ &=& 1
\end{eqnarray*}

Assuming $Fib(n) = \frac{\phi^n - \psi^n}{\sqrt{5}}$ and $Fib(n+1) =
\frac{\phi^{n+1} - \psi^{n+1}}{\sqrt{5}}$ for some $n$,
\begin{eqnarray*}
  Fib(n+2) &=& Fib(n+1) + Fib(n)
        \\ &=& \frac{\phi^{n+1} - \psi^{n+1}}{\sqrt{5}} + \frac{\phi^n - \psi^n}{\sqrt{5}}
        \\ &=& \frac{\phi^n(\phi+1) - \psi^n(\psi+1)}{\sqrt{5}}
        \\ &=& \frac{\phi^n\phi^2 - \psi^n\psi^2}{\sqrt{5}}
        \text{($\phi$ by definition, see below for $\psi$)}
        \\ &=& \frac{\phi^{n+2} - \psi^{n+2}}{\sqrt{5}}
\end{eqnarray*}

$\psi^2 = \psi+1$:
\begin{eqnarray*}
  \psi^2 &=& \left(\frac{1-\sqrt{5}}{2}\right)^2
      \\ &=& \frac{1-2\sqrt{5}+5}{4}
      \\ &=& \frac{3-\sqrt{5}}{2}
      \\ &=& \frac{1-\sqrt{5}}{2} + 1
      \\ &=& \psi + 1
\end{eqnarray*}

% TODO: prove the hint here

Let $F_k(n) = d(Fib(n)+ k, \frac{\phi^n}{\sqrt{5}})$. Then we have
\begin{eqnarray*}
  F_0(n) = d(Fib(n), \frac{\phi^n}{\sqrt{5}}) &=& \left|Fib(n) - \frac{\phi^n}{\sqrt{5}}\right|
  \\ &=& \left|\frac{\phi^n - \psi^n - \phi^n}{\sqrt{5}}\right|
  \\ &=& \left|\frac{\psi^n}{\sqrt{5}}\right|
  \\ F_1(n) = d(Fib(n) + 1, \frac{\phi^n}{\sqrt{5}}) &=& \left|\frac{\psi^n}{\sqrt{5}} + 1\right|
  \\ F_{-1}(n) = d(Fib(n) - 1, \frac{\phi^n}{\sqrt{5}}) &=& \left|\frac{\psi^n}{\sqrt{5}} - 1\right|
\end{eqnarray*}

When $n = 0$:
\begin{eqnarray*}
  d(F_0(0), 0) = \left|\left|\frac{\psi^0}{\sqrt{5}}\right| - 0\right| &=& \frac{1}{\sqrt{5}}
  \\ d(F_1(0), 1) = \left|\left|\frac{\psi^0}{\sqrt{5}} + 1\right| - 1\right| &=& \frac{1}{\sqrt{5}}
  \\ d(F_{-1}(0), 1) = \left|\left|\frac{\psi^0}{\sqrt{5}} - 1\right| - 1\right| &=& \frac{1}{\sqrt{5}}
\end{eqnarray*}

% Since $\frac{1}{\sqrt{5}} < 1 + \frac{1}{\sqrt{5}}$ and $\frac{1}{\sqrt{5}} < 1
% - \frac{1}{\sqrt{5}}$ (as $\frac{1}{\sqrt{5}} < \frac{1}{2}$), we have that
% $F_0(0) < F_1(0)$ and $F_0(0) < F_{-1}(0)$.

% Assuming that $F_0(n) < F_1(n)$ and $F_0(n) < F_{-1}(n)$ for some $n$:

% \begin{eqnarray*}
%   F_0(n+1) &=& \left|\frac{\psi^{n+1}}{\sqrt{5}}\right|
%   \\ &=& \left|\psi\cdot\frac{\psi^{n}}{\sqrt{5}}\right|
%   \\ &<& 
% \end{eqnarray*}

$d(F_0, 0)$, $d(F_1, 1)$ and $d(F_{-1}, 1)$ are monotonically decreasing for all $n$:

\begin{eqnarray*}
  d(F_0(n), 0) &=& \left|\left|\frac{\psi^n}{\sqrt{5}}\right| - 0\right|
            \\ &=& \left|\frac{\psi^n}{\sqrt{5}}\right|
            \\ &>& \left|\frac{\psi^{n+1}}{\sqrt{5}}\right| \text{(since $\psi \in (0,1) \implies \psi^{n+1} < \psi^n$)}
            \\ &=& d(F_0(n+1), 0)
\end{eqnarray*}

\begin{eqnarray*}
  d(F_1(n), 1) &=& \left|\left|\frac{\psi^n}{\sqrt{5}} + 1\right| - 1\right|
            \\ &=& \left|\frac{\psi^n}{\sqrt{5}} + 1 - 1\right| \text{(since $\psi \in (0,1) \implies \frac{\psi^{n+1}}{\sqrt{5}} < \frac{\psi^n}{\sqrt{5}} < \frac{\psi^0}{\sqrt{5}} = \frac{1}{\sqrt{5}} < 1$)}
            \\ &=& \left|\frac{\psi^n}{\sqrt{5}}\right|
            \\ &>& \left|\frac{\psi^{n+1}}{\sqrt{5}}\right| \text{(since $\psi \in (0,1) \implies \psi^{n+1} < \psi^n$)}
            \\ &=& \left|\left|\frac{\psi^{n+1}}{\sqrt{5}} + 1\right| - 1\right| \text{(since $\psi \in (0,1) \implies \frac{\psi^{n+1}}{\sqrt{5}} < \frac{\psi^n}{\sqrt{5}} < \frac{\psi^0}{\sqrt{5}} = \frac{1}{\sqrt{5}} < 1$)}
            \\ &=& d(F_1(n+1), 1)
\end{eqnarray*}

\begin{eqnarray*}
  d(F_{-1}(n), 1) &=& \left|\left|\frac{\psi^n}{\sqrt{5}} - 1\right| - 1\right|
            \\ &=& \left|1 - \frac{\psi^n}{\sqrt{5}} - 1\right| \text{(since $\psi \in (0,1) \implies \frac{\psi^{n+1}}{\sqrt{5}} < \frac{\psi^n}{\sqrt{5}} < \frac{\psi^0}{\sqrt{5}} = \frac{1}{\sqrt{5}} < 1$)}
            \\ &=& \left|\frac{\psi^n}{\sqrt{5}}\right|
            \\ &>& \left|\frac{\psi^{n+1}}{\sqrt{5}}\right| \text{(since $\psi \in (0,1) \implies \psi^{n+1} < \psi^n$)}
            \\ &=& \left|\left|\frac{\psi^{n+1}}{\sqrt{5}} - 1\right| - 1\right| \text{(since $\psi \in (0,1) \implies \frac{\psi^{n+1}}{\sqrt{5}} < \frac{\psi^n}{\sqrt{5}} < \frac{\psi^0}{\sqrt{5}} = \frac{1}{\sqrt{5}} < 1$)}
            \\ &=& d(F_1(n+1), 1)
\end{eqnarray*}

Since $d(F_0(0), 0) = \frac{1}{\sqrt{5}} = d(F_1(0), 1) = d(F_{-1}(0), 1)$ we
know that $Fib(n)$ is closer to $\frac{\phi^n}{\sqrt{5}}$ than either
$Fib(n)+1$ or $Fib(n)-1$ when $n = 0$. Also, since $d(F_0(n), 0)$, $d(F_1(n),
1)$ and $d(F_{-1}(n), 1)$ are all decreasing, the distance between $Fib(n)$ and
$\frac{\phi^n}{\sqrt{5}}$ is decreasing towards $0$, while the distances
between either $Fib(n)+1$ or $Fib(n)-1$ and $\frac{\phi^n}{\sqrt{5}}$ are
decreasing towards 1.
\end{document}
